\documentclass[a4paper,11pt]{report}
\input{notation.inc}
\begin{document}
\noindent\paragraph{Initialization}
\begin{eqnarray}
\mat{G} &=& \mat{d}\transp\mat{d}\\
\vec{a}\iter{0} &=& 0\\
e\iter{0} &=& x\iter{0}\\
w\iter{0} &=& \|\vec{e}\iter{0}\|^2\\
\vec{r}\iter{0} &=& \mat{d}\transp\vec{e}\iter{0}\\
\vec{h}_k\iter{0} &=& \|\mat{d}_k-\vec{e}\iter{0}\|^2 = g_{kk} - 2r_{k}
+ w\iter{0}\\
t &=& 0
\end{eqnarray}
\noindent\paragraph{Loop}
\begin{eqnarray}
j\opt &=& \arg\min_j \left\{ \| \vec{h}_j\iter{t} \| \right\}\\
w\iter{t+1} &=& \vec{h}_{j\opt }\iter{t}\\
%\vec{e}\iter{t+1} &=& \vec{e}\iter{t}-\vec{d}_{k\opt } \\
\vec{r}\iter{t+1} &=& \vec{r}\iter{t} - \vec{g}_{j\opt}\\
h_k\iter{t+1} &=& \|\vec{e}\iter{t} - \vec{d}_k - \vec{d}_{j\opt}\|\\
 &=& \|(\vec{e}\iter{t} - \vec{d}_k) - \vec{d}_{j\opt}\|\\
 &=& [(\vec{e}\iter{t} - \vec{d}_k) -\vec{d}_{j\opt }]\transp[(\vec{e}\iter{t} - \vec{d}_k) -\vec{d}_{j\opt }]\\
 &=& h_k\iter{t} -2\vec{d}_{j\opt }\transp(\vec{e}\iter{t} -
\vec{d}_k) + \vec{d}_{j\opt }\transp\vec{d}_{j\opt }\\
 &=& h_k\iter{t} -2r_{j\opt}\iter{t} +
2g_{kj\opt} + g_{j\opt j\opt} \\
\end{eqnarray}
\end{document}
